Prove SetStateAndUnseal in PB logging library

src/program_proof/simplepb/simplelog/proof.v
@@ -2,6 +2,7 @@ From Perennial.program_proof Require Import grove_prelude.
 From Goose.github_com.mit_pdos.gokv.simplepb Require Export simplelog.
 From Perennial.program_proof Require Import marshal_stateless_proof.
 From coqutil.Datatypes Require Import List.
+From Perennial.goose_lang Require Import crash_borrow.
 
 From Perennial.program_proof.aof Require Import proof.
 
@@ -49,6 +50,14 @@ Lemma file_encodes_state_append op op_bytes data epoch ops :
 Proof.
 Admitted.
 
+Lemma file_encodes_state_snapshot snap ops epoch :
+  has_snap_encoding snap ops →
+  file_encodes_state ((u64_le (length snap) ++ snap) ++ u64_le epoch ++ u64_le (length ops))
+    epoch ops false
+.
+Proof.
+Admitted.
+
 Implicit Types (P:u64 → list OpType → bool → iProp Σ).
 
 Definition file_inv P (contents:list u8) : iProp Σ :=
@@ -74,20 +83,37 @@ Definition is_InMemory_applyVolatileFn (applyVolatileFn:val) own_InMemoryStateMa
   }}}
 .
 
-Definition is_InMemoryStateMachine (sm:loc) own_InMemoryStateMachine : iProp Σ :=
-  ∃ applyVolatileFn,
-  "#HapplyVolatile" ∷ readonly (sm ↦[InMemoryStateMachine :: "ApplyVolatile"] applyVolatileFn) ∗
-  "#HapplyVolatile_spec" ∷ is_InMemory_applyVolatileFn applyVolatileFn own_InMemoryStateMachine
+Definition is_InMemory_setStateFn (setStateFn:val) own_InMemoryStateMachine : iProp Σ :=
+  ∀ ops_prev ops snap snap_sl,
+  {{{
+        ⌜has_snap_encoding snap ops⌝ ∗
+        readonly (is_slice_small snap_sl byteT 1 snap) ∗
+        own_InMemoryStateMachine ops_prev
+  }}}
+    setStateFn (slice_val snap_sl)
+  {{{
+        RET #(); own_InMemoryStateMachine ops
+  }}}
 .
 
-Definition own_StateMachine γaof (s:loc) (epoch:u64) (ops:list OpType) (sealed:bool) P : iProp Σ :=
-  ∃ (fname:string) (aof_ptr:loc) (logsize:u64) (smMem_ptr:loc) data
+Definition is_InMemoryStateMachine (sm:loc) own_InMemoryStateMachine : iProp Σ :=
+  ∃ applyVolatileFn setStateFn,
+  "#HapplyVolatile" ∷ readonly (sm ↦[InMemoryStateMachine :: "ApplyVolatile"] applyVolatileFn) ∗
+  "#HapplyVolatile_spec" ∷ is_InMemory_applyVolatileFn applyVolatileFn own_InMemoryStateMachine ∗
+  "#HsetState" ∷ readonly (sm ↦[InMemoryStateMachine :: "SetState"] setStateFn) ∗
+  "#HsetState_spec" ∷ is_InMemory_setStateFn setStateFn own_InMemoryStateMachine
+.
+
+Definition own_StateMachine (s:loc) (epoch:u64) (ops:list OpType) (sealed:bool) P : iProp Σ :=
+  ∃ (fname:string) (aof_ptr:loc) γaof (logsize:u64) (smMem_ptr:loc) data
     own_InMemoryStateMachine,
     "Hfname" ∷ s ↦[StateMachine :: "fname"] #(LitString fname) ∗
     "HlogFile" ∷ s ↦[StateMachine :: "logFile"] #aof_ptr ∗
     "HsmMem" ∷ s ↦[StateMachine :: "smMem"] #smMem_ptr ∗
     "HnextIndex" ∷ s ↦[StateMachine :: "nextIndex"] #(U64 (length ops)) ∗
     "Hlogsize" ∷ s ↦[StateMachine :: "logsize"] #logsize ∗
+    "Hepoch" ∷ s ↦[StateMachine :: "epoch"] #epoch ∗
+    "Hsealed" ∷ s ↦[StateMachine :: "sealed"] #sealed ∗
 
     "Haof" ∷ aof_log_own γaof data ∗
     "#His_aof" ∷ is_aof aof_ptr γaof fname (file_inv P) ∗
@@ -97,19 +123,19 @@ Definition own_StateMachine γaof (s:loc) (epoch:u64) (ops:list OpType) (sealed:
     (* "HsmMem" ∷ *)
 .
 
-Lemma StateMachine__apply s Q (op:OpType) (op_bytes:list u8) op_sl γaof epoch ops P :
+Lemma StateMachine__apply s Q (op:OpType) (op_bytes:list u8) op_sl epoch ops P :
   {{{
         ⌜has_op_encoding op_bytes op⌝ ∗
         readonly (is_slice_small op_sl byteT 1 op_bytes) ∗
         (P epoch ops false ={⊤}=∗ P epoch (ops ++ [op]) false ∗ Q) ∗
-        own_StateMachine γaof s epoch ops false P
+        own_StateMachine s epoch ops false P
   }}}
     StateMachine__apply #s (slice_val op_sl)
   {{{
         reply_sl q (waitFn:goose_lang.val),
         RET (slice_val reply_sl, waitFn);
         is_slice_small reply_sl byteT q (compute_reply ops op) ∗
-        own_StateMachine γaof s epoch (ops ++ [op]) false P ∗
+        own_StateMachine s epoch (ops ++ [op]) false P ∗
         (∀ Ψ, (Q -∗ Ψ #()) -∗ WP waitFn #() {{ Ψ }})
   }}}
 .
@@ -204,7 +230,7 @@ Proof.
   iFrame.
   iSplitR "HupdQ".
   {
-    iExists _, _, _, _, _, _.
+    iExists _, _, _, _, _, _, _.
     iFrame "∗#".
     iSplitL; last first.
     { iPureIntro. by apply file_encodes_state_append. }
@@ -225,5 +251,179 @@ Proof.
   iApply "HΨ".
   iFrame.
 Admitted.
+
+Opaque crash_borrow.
+Lemma wp_SetStateAndUnseal s (set_state_fn:val) P ops_prev (epoch_prev:u64) sealed_prev ops epoch (snap:list u8) snap_sl Q :
+  {{{
+        ⌜has_snap_encoding snap ops⌝ ∗
+        readonly (is_slice_small snap_sl byteT 1 snap) ∗
+        (P epoch_prev ops_prev sealed_prev ={⊤}=∗ P epoch ops false ∗ Q) ∗
+        own_StateMachine s epoch_prev ops_prev sealed_prev P
+  }}}
+    StateMachine__setStateAndUnseal #s (slice_val snap_sl) #(U64 (length ops)) #epoch
+  {{{
+        RET #();
+        own_StateMachine s epoch ops false P ∗ Q
+  }}}
+.
+Proof.
+  iIntros (Φ) "(%HsnapEnc & #Hsnap_sl & Hupd & Hown) HΦ".
+  wp_lam.
+  wp_pures.
+  iNamed "Hown".
+
+  wp_storeField.
+  wp_storeField.
+  wp_storeField.
+
+  iAssert (_) with "HisMemSm" as "#HisMemSm2".
+  iNamed "HisMemSm2".
+  wp_loadField.
+  wp_loadField.
+  wp_apply ("HsetState_spec" with "[$Hsnap_sl $Hmemstate]").
+  { done. }
+  iIntros "Hmemstate".
+
+  wp_pures.
+
+  (* XXX: this could be a separate lemma *)
+  wp_lam.
+  wp_pures.
+
+  (* create contents of brand new file *)
+
+  wp_apply (wp_slice_len).
+  wp_apply (wp_NewSliceWithCap).
+  { apply encoding.unsigned_64_nonneg. }
+
+  iIntros (?) "Henc_sl".
+  wp_apply (wp_ref_to).
+  { done. }
+  iIntros (enc_ptr) "Henc".
+  wp_pures.
+  wp_apply (wp_slice_len).
+  wp_load.
+  wp_apply (wp_WriteInt with "[$Henc_sl]").
+  iIntros (enc_sl) "Henc_sl".
+  wp_pures.
+  wp_store.
+
+  wp_load.
+  iMod (readonly_load with "Hsnap_sl") as (?) "Hsnap_sl2".
+  iDestruct (is_slice_small_sz with "Hsnap_sl2") as "%Hsnap_sz".
+  wp_apply (wp_WriteBytes with "[$Henc_sl $Hsnap_sl2]").
+  iIntros (enc_sl2) "[Henc_sl _]".
+  wp_store.
+
+  wp_loadField.
+  wp_load.
+  wp_apply (wp_WriteInt with "[$Henc_sl]").
+  iIntros (enc_sl3) "Henc_sl".
+  wp_pures.
+  wp_store.
+
+  wp_loadField.
+  wp_load.
+  wp_apply (wp_WriteInt with "[$Henc_sl]").
+  iIntros (enc_sl4) "Henc_sl".
+  wp_pures.
+  wp_store.
+
+  replace (int.nat 0) with (0%nat) by word.
+  rewrite replicate_0.
+  rewrite app_nil_l.
+  replace (snap_sl.(Slice.sz)) with (U64 (length snap)); last first.
+  { word. }
+
+  wp_loadField.
+  wp_pures.
+
+  wp_loadField.
+
+  wp_apply (wp_AppendOnlyFile__Close with "His_aof [$Haof]").
+  iIntros "Hfile".
+  wp_pures.
+
+  wp_load.
+  wp_loadField.
+
+  wp_bind (FileWrite _ _).
+  iApply (wpc_wp _ _ _ _ True).
+
+  wpc_apply (wpc_crash_borrow_open_modify with "Hfile").
+  { done. }
+  iSplit; first done.
+  iIntros "[Hfile Hinv]".
+  iDestruct (is_slice_to_small with "Henc_sl") as "Henc_sl".
+  iApply wpc_fupd.
+  wpc_apply (wpc_FileWrite with "[$Hfile $Henc_sl]").
+  iSplit.
+  { (* case: crash; *)
+    iIntros "[Hbefore|Hafter]".
+    {
+      iSplitR; first done.
+      iModIntro; iExists _; iFrame.
+    }
+    { (* fire update; this is the same as the reasoning in the non-crash case *)
+      iSplitR; first done.
+
+      iDestruct "Hinv" as (???) "[%Henc2 HP]".
+      pose proof (file_encodes_state_inj _ _ _ _ _ _ _ Henc2 Henc) as [-> [-> ->]].
+      iMod ("Hupd" with "HP") as "[HP _]".
+      iModIntro. iExists _; iFrame.
+      iExists _, _, _; iFrame "HP".
+      iPureIntro.
+      rewrite -app_assoc.
+      by apply file_encodes_state_snapshot.
+    }
+  }
+  iNext.
+  iIntros "[Hfile _]".
+  iExists _.
+
+  (* update file_inv *)
+  iDestruct "Hinv" as (???) "[%Henc2 HP]".
+  pose proof (file_encodes_state_inj _ _ _ _ _ _ _ Henc2 Henc) as [-> [-> ->]].
+  iMod ("Hupd" with "HP") as "[HP HQ]".
+  iModIntro.
+  rewrite -app_assoc.
+  set (newdata:=(u64_le (length snap) ++ snap) ++ u64_le epoch ++ u64_le (length ops)).
+  iAssert (file_inv P newdata) with "[HP]" as "HP".
+  {
+    iExists _, _, _; iFrame "HP".
+    iPureIntro.
+    unfold newdata.
+    rewrite -app_assoc.
+    by apply file_encodes_state_snapshot.
+  }
+  iSplitL "Hfile HP".
+  { iAccu. }
+  iSplit.
+  {
+    iModIntro.
+    iIntros "[Hfile HP]".
+    iModIntro. iExists _; iFrame.
+  }
+  iIntros "Hfile".
+  iSplit; first done.
+  wp_pures.
+  wp_loadField.
+
+  wp_apply (wp_CreateAppendOnlyFile _ _ (file_inv P) with "[$Hfile]").
+  iClear "His_aof".
+  iIntros (new_aof_ptr γaof2) "[His_aof Haof]".
+  wp_storeField.
+  wp_pures.
+  iApply "HΦ".
+  iFrame "HQ".
+  iModIntro.
+  iExists fname, new_aof_ptr, γaof2, _, _, newdata, own_InMemoryStateMachine.
+  iFrame "∗".
+  iFrame "#".
+  iPureIntro.
+  unfold newdata.
+  rewrite -app_assoc.
+  by apply file_encodes_state_snapshot.
+Qed.
 
 End proof.
